universe consistent definitions.

theories/Views/FuncView.v
@@ -1,4 +1,5 @@
 Require Import ExtLib.Tactics.
+Require Import ExtLib.Data.POption.
 Require Import MirrorCore.Views.Ptrns.
 Require Import MirrorCore.TypesI.
 Require Import MirrorCore.SymI.
@@ -7,45 +8,41 @@ Require Import MirrorCore.syms.SymOneOf.
 Set Implicit Arguments.
 Set Strict Implicit.
 Set Maximal Implicit Insertion.
-
-Inductive view_option (A : Type) :=
-  | vSome : A -> view_option A
-  | vNone : view_option A.
-
-Implicit Arguments vNone [[A]].
+Set Printing Universes.
 
 Section FuncView.
-  Variables func A : Type.
+  Polymorphic Universes s t.
+  Polymorphic Variables func A : Type@{s}.
 
-  Class FuncView : Type :=
+  Polymorphic Class FuncView : Type@{s} :=
   { f_insert : A -> func
-  ; f_view : func -> view_option A
+  ; f_view : func -> poption A
   }.
 
-  Variable FV : FuncView.
+  Polymorphic Variable FV : FuncView.
 
-  Variable typ : Type.
-  Variable RType_typ : RType typ.
-  Variable Sym_func : RSym func.
-  Variable Sym_A : RSym A.
+  Polymorphic Variable typ : Type@{t}.
+  Polymorphic Variable RType_typ : RType typ.
+  Polymorphic Variable Sym_func : RSym func.
+  Polymorphic Variable Sym_A : RSym A.
 
-  Class FuncViewOk : Type :=
-  { fv_ok : forall f a, f_view f = vSome a <-> f_insert a = f
+  Polymorphic Class FuncViewOk : Type :=
+  { fv_ok : forall f a, f_view f = pSome a <-> f_insert a = f
   ; fv_compat : forall (a : A) t,
       symAs a t = symAs (f_insert a) t
   }.
 
-  Lemma fv_okL {FVO : FuncViewOk} f a (H : f_view f = vSome a) :
+  Polymorphic Lemma fv_okL {FVO : FuncViewOk} f a (H : f_view f = pSome a) :
     f_insert a = f.
-  Proof.
+  Proof using.
     apply fv_ok; assumption.
   Qed.
 
-  Variable RTypeOk_typ : RTypeOk.
+  Polymorphic Variable RTypeOk_typ : RTypeOk.
 
-  Theorem fv_compat_typ (FVO : FuncViewOk)
+  Polymorphic Theorem fv_compat_typ (FVO : FuncViewOk)
   : forall a, typeof_sym (f_insert a) = typeof_sym a.
-  Proof.
+  Proof using RTypeOk_typ.
     intros.
     generalize (fv_compat a).
     unfold symAs. intros.
@@ -70,7 +67,7 @@ Section FuncView.
       eauto. }
   Defined.
 
-  Theorem fv_compat_val (FVO : FuncViewOk)
+  Polymorphic Theorem fv_compat_val (FVO : FuncViewOk)
   : forall (a : A),
         symD a = match fv_compat_typ _ a in _ = T return match T with
                                                          | Some t => typD t
@@ -79,7 +76,7 @@ Section FuncView.
                  with
                  | eq_refl => symD (f_insert a)
                  end.
-  Proof.
+  Proof using.
     intros.
     assert (typeof_sym a = None \/ exists t, typeof_sym a = Some t).
     { clear. destruct (typeof_sym a); eauto. }
@@ -103,10 +100,10 @@ Section FuncView.
       inv_all. assumption. }
   Qed.
 
-  Lemma fv_typeof_sym {FVO : FuncViewOk} f p t v
-    (Hview : f_view f = vSome p) (Hfunc : symAs f t = Some v) :
+  Polymorphic Lemma fv_typeof_sym {FVO : FuncViewOk} f p t v
+    (Hview : f_view f = pSome p) (Hfunc : symAs f t = Some v) :
     typeof_sym p = Some t.
-  Proof.
+  Proof using.
     destruct (fv_ok f p) as [H _].
     specialize (H Hview); subst.
     rewrite <- fv_compat in Hfunc.
@@ -116,14 +113,38 @@ Section FuncView.
     forward.
   Defined.
 
-  Definition ptrn_view {T} (p : ptrn A T) : ptrn func T :=
+  Polymorphic Variable FVO : FuncViewOk.
+
+  Global Polymorphic Instance Injective_exprD'_f_insert (a : A) (t : typ) (v : typD t)
+  : Injective (symAs (f_insert a) t = Some v) :=
+  { result := symAs a t = Some v
+  ; injection := fun H => _
+  }.
+  Proof.
+    rewrite fv_compat; assumption.
+  Defined.
+
+  Polymorphic Lemma symAs_finsertI (t : typ) (f : A)
+        (P : option (typD t) -> Prop)
+        (H : P (symAs f t)) :
+    P (symAs (f_insert f) t).
+  Proof.
+    rewrite <- fv_compat; assumption.
+  Qed.
+
+  Section ptrns.
+  Polymorphic Universe X L.
+  Context {T : Type@{X}}.
+
+  Polymorphic Definition ptrn_view (p : ptrn@{X X L} A T)
+  : ptrn@{s X L} func T :=
     fun e _T good bad =>
       match f_view e with
-      | vNone => bad e
-      | vSome f => p f _T good (fun _ => bad e)
+      | pNone => bad e
+      | pSome f => p f _T good (fun _ => bad e)
       end.
 
-  Global Instance ptrn_view_ok T (p : ptrn A T)
+  Global Polymorphic Instance ptrn_view_ok (p : ptrn A T)
   : ptrn_ok p -> ptrn_ok (ptrn_view p).
   Proof.
     unfold ptrn_view, ptrn_ok, Succeeds, Fails.
@@ -137,12 +158,10 @@ Section FuncView.
     { eauto. }
   Qed.
 
-  Variable FVO : FuncViewOk.
-
-  Theorem Succeeds_ptrn_view {T} (p : ptrn A T) x res (H : ptrn_ok p)
+  Polymorphic Theorem Succeeds_ptrn_view (p : ptrn A T) x res (H : ptrn_ok p)
   : Succeeds x (ptrn_view p) res ->
     exists f, f_insert f = x /\ Succeeds f p res.
-  Proof.
+  Proof using RTypeOk_typ Sym_func Sym_A FVO.
     unfold Succeeds, ptrn_view. intros.
     destruct (f_view x) eqn:Heq.
     { eapply fv_ok in Heq.
@@ -156,29 +175,14 @@ Section FuncView.
       specialize (H0 _ (fun _ => true) (fun _ => false)); inversion H0. }
   Qed.
 
-  Global Instance ptrn_view_SucceedsE {T : Type} {x : func} {res : T} {p : ptrn A T} 
+  Global Polymorphic Instance ptrn_view_SucceedsE
+         {x : func} {res : T} {p : ptrn A T} 
          {Sym_A : RSym A}
          {pok : ptrn_ok p}
   : SucceedsE x (ptrn_view p) res :=
   { s_result := exists f : A, f_insert f = x /\ Succeeds f p res
-  ; s_elim := @Succeeds_ptrn_view T p x res _
+  ; s_elim := @Succeeds_ptrn_view p x res _
   }.
-
-  Global Instance Injective_exprD'_f_insert (a : A) (t : typ) (v : typD t)
-  : Injective (symAs (f_insert a) t = Some v) :=
-  { result := symAs a t = Some v
-  ; injection := fun H => _
-  }.
-  Proof.
-    rewrite fv_compat; assumption.
-  Defined.
-
-  Lemma symAs_finsertI (t : typ) (f : A)
-        (P : option (typD t) -> Prop)
-        (H : P (symAs f t)) :
-    P (symAs (f_insert f) t).
-  Proof.
-    rewrite <- fv_compat; assumption.
-  Qed.
+  End ptrns.
 
 End FuncView.
